library/init/meta/occurrences.lean
@@ -25,6 +25,11 @@ inductive occurrences
 
 open occurrences
 
+def occurrences.contains : occurrences → nat → bool
+| all                  p := tt
+| (occurrences.pos ps) p := to_bool (p ∈ ps)
+| (occurrences.neg ps) p := to_bool (p ∉ ps)
+
 instance : inhabited occurrences :=
 ⟨all⟩
 
