tests/lean/unfold_crash.lean
@@ -4,7 +4,10 @@ open nat tactic
 example (a b : nat) : a = succ b → a = b + 1 :=
 by do
   H ← intro `H,
-  try (unfold_at [`nat.succ] H),
-  unfold [`add], dsimp, unfold [`nat.add],
+  try (dunfold_at [`nat.succ] H),
+  dunfold [`add, `has_add.add, `has_one.one, `nat.add, `one],
   trace_state,
+  t ← target,
+  expected ← to_expr `(a = succ b),
+  guard (t = expected),
   assumption
